src/Core/IntPtrLemmas.v
@@ -13,6 +13,136 @@ Proof.
 Qed.
 
 
+Proposition distance_to_sem_cmp_lt : forall dist m b1 b2 i1 i2,
+    distance m (b1, i1) (b2, i2) = Some (S dist) ->
+    sem_cmp Clt (Vptr b1 i1) (tptr tschar)
+            (Vptr b2 i2) (tptr tschar) m = Some Vtrue.
+Proof.
+  intros until i2; intro Dist.
+  replace b1 with b2 in *.
+  pose proof (dist_to_lt _ _ _ _ _ Dist) as LT.
+  unfold distance, sem_cmp, cmp_ptr, addr_ge, ptr_ge,
+  Val.cmplu_bool, Val.cmpu_bool, Ptrofs.cmpu,
+  Val.cmp_different_blocks,
+  classify_cmp in *.
+  repeat break_match;
+    try congruence; repeat destruct_andb_hyp;
+      try congruence.
+  all: try rewrite <- ptrofs_lt_signed_lt in LT;
+    try bool_rewrite; try intuition.
+  unfold sem_binarith.
+  all: repeat break_match; simpl in *; try congruence.
+  
+  simpl in *.
+  all: unfold classify_cmp in *.
+
+  unfold distance, sem_cmp, cmp_ptr, addr_ge, ptr_ge,
+  Val.cmplu_bool, Val.cmpu_bool, Ptrofs.cmpu,
+  Val.cmp_different_blocks,
+  classify_cmp in *.
+  repeat break_match;
+    try congruence; repeat destruct_andb_hyp;
+      try congruence.
+Qed.
+
+Lemma dist_succ : forall m b b' ofs ofs' dist,
+    distance m (b', ofs') (b, ofs) = Some (S dist) ->
+    Mem.weak_valid_pointer m b' (Ptrofs.unsigned (ofs' + 1)%ptrofs) = true -> 
+    distance m (b', (Ptrofs.add ofs' Ptrofs.one)) (b, ofs) = Some dist.
+Proof.
+  unfold distance, snd; intros.
+  break_match_hyp; [| discriminate].
+  break_if; subst; [| discriminate].
+  inversion H; clear H.
+  assert (Ptrofs.unsigned ofs' < Ptrofs.max_unsigned)%Z.
+  {
+    assert ((Ptrofs.unsigned ofs') < (Ptrofs.unsigned ofs))%Z.
+    {
+      assert ((Z.to_nat (Ptrofs.unsigned ofs') 
+               < 
+               Z.to_nat (Ptrofs.unsigned ofs))%nat) by lia.
+      unfold Ptrofs.unsigned in *.
+      destruct ofs, ofs'; simpl in *.
+      pose proof (Z2Nat.inj_lt intval0 intval) as Inj.
+      destruct Inj.
+      all: try lia.
+    }
+    assert (Ptrofs.unsigned ofs <= Ptrofs.max_unsigned)%Z.
+    pose proof (Ptrofs.unsigned_range_2 ofs).
+    all: try lia.
+  }
+  replace (addr_ge m (b, ofs) (b', (ofs' + 1)%ptrofs))
+    with (Some true).
+  f_equal.
+  enough (S (Z.to_nat (Ptrofs.unsigned (ofs')%ptrofs)) =
+             Z.to_nat (Ptrofs.unsigned (ofs' + 1)%ptrofs)) by lia.
+  rewrite Ptrofs.add_unsigned, Ptrofs.unsigned_repr, <-Z2Nat.inj_succ.
+  reflexivity.
+  apply Ptrofs.unsigned_range.
+  replace (Ptrofs.unsigned 1%ptrofs) with 1 by reflexivity.
+  pose proof Ptrofs.unsigned_range ofs'.
+  lia.
+
+  unfold addr_ge, ptr_ge in *.
+  simpl in *.
+  repeat break_if; subst.
+  all: try discriminate; unfold Mem.weak_valid_pointer in *.
+  all: repeat destruct_andb_hyp.
+  all: repeat destruct_orb_hyp.
+  all: try congruence.
+  all: clear - H H2 Heqo.
+
+  all: assert (Z.to_nat (Ptrofs.unsigned ofs') + 1 <=
+          Z.to_nat (Ptrofs.unsigned ofs))%nat
+    by lia.
+  all: unfold Ptrofs.ltu.
+  all: break_if.
+  all: rewrite Ptrofs.add_unsigned, Ptrofs.unsigned_repr in *.
+  all: replace (Ptrofs.unsigned 1%ptrofs) with 1 in * by reflexivity.
+  all: replace (1)%nat with (Z.to_nat 1)%nat in H0 by reflexivity.
+  all: rewrite <-Z2Nat.inj_add in H0.
+  all: try rewrite <-Z2Nat.inj_le in H0.
+  all: try apply Ptrofs.unsigned_range.
+  all: try reflexivity.
+  all: replace (Ptrofs.unsigned 1%ptrofs) with 1 by reflexivity.
+  all: pose proof Ptrofs.unsigned_range ofs'.
+  all: try lia.
+Qed.
+
+Proposition distance_succ_no_overflow :  forall m b b' ofs ofs' dist,
+    distance m (b', ofs') (b, ofs) = Some (S dist) ->
+    Ptrofs.unsigned (ofs' + 1)%ptrofs = Ptrofs.unsigned ofs' + 1.
+Proof.
+  intros.
+  unfold distance, snd in *; intros.
+  break_match_hyp; [| discriminate].
+  break_if; subst; [| discriminate].
+  inversion H; clear H.
+  assert (Ptrofs.unsigned ofs' < Ptrofs.max_unsigned)%Z.
+  {
+    assert ((Ptrofs.unsigned ofs') < (Ptrofs.unsigned ofs))%Z.
+    {
+      assert ((Z.to_nat (Ptrofs.unsigned ofs') 
+               < 
+               Z.to_nat (Ptrofs.unsigned ofs))%nat) by lia.
+      unfold Ptrofs.unsigned in *.
+      destruct ofs, ofs'; simpl in *.
+      pose proof (Z2Nat.inj_lt intval0 intval) as Inj.
+      destruct Inj.
+      all: try lia.
+    }
+    assert (Ptrofs.unsigned ofs <= Ptrofs.max_unsigned)%Z.
+    pose proof (Ptrofs.unsigned_range_2 ofs).
+    all: try lia.
+  }
+  
+  all: rewrite Ptrofs.add_unsigned, Ptrofs.unsigned_repr in *.
+  all: replace (Ptrofs.unsigned 1%ptrofs) with 1 in * by reflexivity.
+  auto.
+  destruct ofs'; simpl in *.
+  nia.
+Qed.
+
 Proposition distance_O : forall m b1 b2 i1 i2,
     distance m (b1,i1) (b2,i2) = Some O <->
     ((b1,i1) = (b2,i2))%ptrofs
@@ -98,7 +228,7 @@ Qed.
 
 Proposition addr_lt_ge_eq : forall b m b1 b2 i1 i2 ,
     addr_ge m (b1, i1) (b2, i2) = Some b
-    <-> addr_lt m (b2, i2) (b1, i1) = Some (negb b).
+    <-> addr_lt m (b1, i1) (b2, i2) = Some (negb b).
 Proof.
   intros.
   unfold addr_lt.
@@ -116,21 +246,118 @@ Proof.
     all: try congruence.  
 Qed.
 
-Proposition addr_lt_to_sem_cmp_lt : forall m b1 b2 i1 i2,
-  addr_lt m (b1, i1) (b2, i2) = Some false ->
-     (sem_cmp Clt (Vptr b1 i1) (tptr tschar)
-              (Vptr b2 i2) (tptr tschar) m = Some (Val.of_bool false)).
+Proposition addr_lt_ge_eq' : forall b m b1 b2 i1 i2 ,
+    addr_lt m (b1, i1) (b2, i2) = Some b
+    <-> addr_ge m (b1, i1) (b2, i2) = Some (negb b).
 Proof.
-Admitted.
+  intros.
+  unfold addr_lt.
+  simpl.
+  destruct b.
+  * unfold option_map.
+    break_match.
+    destruct b.
+    all: try (intuition || congruence).
+    all: try congruence.
+  * unfold option_map.
+    break_match.
+    destruct b.
+    all: try (intuition || congruence).
+    all: try congruence.  
+Qed.
 
-Proposition addr_lt_succ_to_sem_cmp_lt : forall m b1 b2 i1 i2,
-  addr_lt m (b1,(i1 + 1)%ptrofs) (b2, i2) = Some true ->
-     (sem_cmp Clt (Vptr b1 i1) (tptr tschar)
-              (Vptr b2 i2) (tptr tschar) m = Some Vtrue).
-Admitted.
+Proposition addr_ge_to_ge : forall b m b1 b2 i1 i2 ,
+    addr_ge m (b1, i1) (b2, i2) = Some b
+    -> (i2 <=u i1)%ptrofs = b.
+Proof.
+  intros.
+  unfold distance, sem_cmp, cmp_ptr, addr_lt, addr_ge, ptr_ge,
+  Val.cmplu_bool, Val.cmpu_bool, Ptrofs.cmpu,
+  Val.cmp_different_blocks,
+  classify_cmp in *.
+  repeat break_match;
+    try congruence;
+      simpl in *;
+      try congruence.
+Qed.
 
-Proposition dist_succ_to_sem_cmp_lt : forall dist m b1 b2 i1 i2,
-    distance m (b1, i1) (b2, i2) = Some (S dist) ->
+Proposition addr_lt_to_lt : forall b m b1 b2 i1 i2 ,
+    addr_lt m (b1, i1) (b2, i2) = Some b
+    -> (i1 <u i2)%ptrofs = b.
+Proof.
+  intros.
+  unfold addr_lt in *.
+  Locate addr_lt.
+  unfold distance, sem_cmp, cmp_ptr, addr_lt, addr_ge, ptr_ge,
+  Val.cmplu_bool, Val.cmpu_bool, Ptrofs.cmpu,
+  Val.cmp_different_blocks,
+  classify_cmp in *.
+  repeat break_match;
+    try congruence;
+      simpl in *;
+      try congruence;
+      try intuition.
+  unfold Ptrofs.ltu in *.
+  repeat break_match;
+    simpl in *;
+    try congruence;
+    try nia.
+Qed.
+
+Proposition addr_lt_to_sem_cmp_lt : forall b m b1 b2 i1 i2,
+  addr_lt m (b1, i1) (b2, i2) = Some b ->
      (sem_cmp Clt (Vptr b1 i1) (tptr tschar)
-              (Vptr b2 i2) (tptr tschar) m = Some Vtrue).
-  Admitted.
+              (Vptr b2 i2) (tptr tschar) m = Some (Val.of_bool b)).
+Proof.
+  intros until i2; intro Addr.
+  eapply sem_Clt_Cge_ptr'.
+  eapply addr_lt_ge_eq' in Addr.
+   eapply ptr_ge_to_sem_cmp;
+     eassumption.
+Qed.
+
+Proposition addr_lt_trans : forall m b1 b2 i1 i2,
+    addr_lt m (b1, (i1 + 1)%ptrofs) (b2, i2) = Some true ->
+    Ptrofs.unsigned (i1 + 1)%ptrofs = Ptrofs.unsigned i1 + 1 ->
+    Mem.weak_valid_pointer m b1 (Ptrofs.unsigned i1) = true ->
+    addr_lt m (b1, i1) (b2, i2) = Some true.
+Proof.
+  intros until i2;
+    intro Addr; intro OF;
+      intro Ptr.
+  unfold addr_lt, Mem.weak_valid_pointer in *.
+  unfold distance, sem_cmp, cmp_ptr, addr_lt, addr_ge, ptr_ge,
+  Val.cmplu_bool, Val.cmpu_bool, Ptrofs.cmpu,
+  Val.cmp_different_blocks,
+  classify_cmp in *.
+  repeat break_match;
+    try congruence;
+    simpl in *;
+    try congruence;
+    try intuition.
+  unfold Ptrofs.ltu in *.
+  repeat break_match;
+    simpl in *;
+    try congruence;
+    rewrite OF in *;
+    simpl in *;
+    try nia.
+  repeat destruct_andb_hyp;
+    repeat destruct_orb_hyp;
+    try congruence.
+  Qed.
+  
+Proposition addr_lt_succ_to_sem_cmp : forall m b1 b2 i1 i2,
+    addr_lt m (b1, (i1 + 1)%ptrofs) (b2, i2) = Some true ->
+    Ptrofs.unsigned (i1 + 1)%ptrofs = Ptrofs.unsigned i1 + 1 ->
+    Mem.weak_valid_pointer m b1 (Ptrofs.unsigned i1) = true ->
+    (sem_cmp Clt (Vptr b1 i1) (tptr tschar)
+             (Vptr b2 i2) (tptr tschar) m = Some (Val.of_bool true)).
+Proof.
+  intros until i2;
+    intro Addr; intro OF; intro Ptr.
+  eapply addr_lt_trans in Addr.
+  eapply addr_lt_to_sem_cmp_lt.
+  all: eassumption.
+Qed.
+
